src/Binary_tree.v
@@ -7,13 +7,14 @@ Set Implicit Arguments.
 
 Module Make (ElementM:ANY) (ExtraM:ANY).
 
-  Definition A := ElementM.T.
-  Definition E := ExtraM.T.
+  Module A := ElementM.
+  Module E := ExtraM.
+
 
 (** * List *)
 (*    ==== *)
   Module List.
-    Definition L: Set := list A.
+    Definition L: Set := list A.t.
 
     Inductive Permutation: L -> L -> Prop :=
     | perm_empty:
@@ -32,101 +33,101 @@ Module Make (ElementM:ANY) (ExtraM:ANY).
   (** * Basic Definitions               *)
   (*====================================*)
   Section basic_definitions.
-    Inductive T: Set :=
-    | empty: T
-    | node:  A -> E -> T -> T -> T.
+    Inductive t: Set :=
+    | Empty: t
+    | Node:  A.t -> E.t -> t -> t -> t.
 
-    Definition Node (t:T): Prop :=
-      match t with
-      | empty => False
-      | node _ _ _ _ => True
+    Definition is_Node (t_:t): Prop :=
+      match t_ with
+      | Empty => False
+      | Node _ _ _ _ => True
       end.
 
     Theorem node_not_empty:
-      forall(a:A) (i:E) (t1 t2: T),
-        node a i t1 t2 <> empty.
+      forall(a:A.t) (i:E.t) (t1 t2: t),
+        Node a i t1 t2 <> Empty.
     Proof
       fun a i t1 t2 p =>
-        Equal.rewrite p Node I.
+        Equal.rewrite p is_Node I.
 
-    Definition is_node (t:T): {Node t} + {~ Node t} :=
-      match t return {Node t} + {~ Node t} with
-        empty => right (fun p:False => match p with end)
-      | node _ _ _ _ => left I
+    Definition is_node (t_:t): {is_Node t_} + {~ is_Node t_} :=
+      match t_ return {is_Node t_} + {~ is_Node t_} with
+        Empty => right (fun p:False => match p with end)
+      | Node _ _ _ _ => left I
       end.
 
-    Inductive Element: T -> A -> Prop :=
+    Inductive Element: t -> A.t -> Prop :=
     | element_node:
-        forall a e t1 t2, Element (node a e t1 t2) a.
+        forall a e t1 t2, Element (Node a e t1 t2) a.
 
-    Inductive Extra: T -> E -> Prop :=
+    Inductive Extra: t -> E.t -> Prop :=
     | extra_node:
-        forall a e t1 t2, Extra (node a e t1 t2) e.
+        forall a e t1 t2, Extra (Node a e t1 t2) e.
 
-    Theorem extra_is_node: forall (t:T) (e:E), Extra t e -> Node t.
+    Theorem extra_is_node: forall (t_:t) (e:E.t), Extra t_ e -> is_Node t_.
     Proof
       fun t e extra =>
-        match extra in Extra t _ return Node t with
+        match extra in Extra t _ return is_Node t with
         | extra_node a e t1 t2 => I
         end.
 
-    Definition left_son (t:T): Node t -> T :=
-      match t with
-      | empty => fun nd => match nd with end
-      | node a e t1 t2 => fun _ => t1
+    Definition left_son (t_:t): is_Node t_ -> t :=
+      match t_ with
+      | Empty => fun nd => match nd with end
+      | Node a e t1 t2 => fun _ => t1
       end.
 
-    Definition right_son (t:T): Node t -> T :=
-      match t with
-      | empty => fun nd => match nd with end
-      | node a e t1 t2 => fun _ => t2
+    Definition right_son (t_:t): is_Node t_ -> t :=
+      match t_ with
+      | Empty => fun nd => match nd with end
+      | Node a e t1 t2 => fun _ => t2
       end.
 
-    Definition element (t:T): Node t -> A :=
-      match t with
-      | empty => fun nd => match nd with end
-      | node a e t1 t2 => fun _ => a
+    Definition element (t_:t): is_Node t_ -> A.t :=
+      match t_ with
+      | Empty => fun nd => match nd with end
+      | Node a e t1 t2 => fun _ => a
       end.
 
-    Definition extra (t:T): Node t -> E :=
-      match t with
-      | empty => fun nd => match nd with end
-      | node a e t1 t2 => fun _ => e
+    Definition extra (t_:t): is_Node t_ -> E.t :=
+      match t_ with
+      | Empty => fun nd => match nd with end
+      | Node a e t1 t2 => fun _ => e
       end.
 
     Theorem left_son_correct:
-      forall (a:A) (e:E) (t1 t2:T),
-        t1 = left_son (node a e t1 t2) I.
+      forall (a:A.t) (e:E.t) (t1 t2:t),
+        t1 = left_son (Node a e t1 t2) I.
     Proof
       fun a e t1 t2 => eq_refl.
 
     Theorem right_son_correct:
-      forall (a:A) (e:E) (t1 t2:T),
-        t2 = right_son (node a e t1 t2) I.
+      forall (a:A.t) (e:E.t) (t1 t2:t),
+        t2 = right_son (Node a e t1 t2) I.
     Proof
       fun a e t1 t2 => eq_refl.
 
     Theorem element_correct:
-      forall (a:A) (e:E) (t1 t2:T),
-        a = element (node a e t1 t2) I.
+      forall (a:A.t) (e:E.t) (t1 t2:t),
+        a = element (Node a e t1 t2) I.
     Proof
       fun a e t1 t2 => eq_refl.
 
     Theorem extra_correct:
-      forall (a:A) (e:E) (t1 t2:T),
-        e = extra (node a e t1 t2) I.
+      forall (a:A.t) (e:E.t) (t1 t2:t),
+        e = extra (Node a e t1 t2) I.
     Proof
       fun a e t1 t2 => eq_refl.
 
     Theorem node_injective_extra:
-      forall (a1 a2:A) (e1 e2:E) (t11 t12 t21 t22:T),
-        node a1 e1 t11 t12 = node a2 e2 t21 t22 ->
+      forall (a1 a2:A.t) (e1 e2:E.t) (t11 t12 t21 t22:t),
+        Node a1 e1 t11 t12 = Node a2 e2 t21 t22 ->
         e1 = e2.
     Proof
       let f e0 t :=
           match t with
-          | empty => e0
-          | node a e t1 t2 => e
+          | Empty => e0
+          | Node a e t1 t2 => e
           end
       in
       fun a1 a2 e1 e2 t11 t12 t21 t22 eq =>
@@ -135,14 +136,14 @@ Module Make (ElementM:ANY) (ExtraM:ANY).
           (f e1).
 
     Theorem node_injective_element:
-      forall (a1 a2:A) (e1 e2:E) (t11 t12 t21 t22:T),
-        node a1 e1 t11 t12 = node a2 e2 t21 t22 ->
+      forall (a1 a2:A.t) (e1 e2:E.t) (t11 t12 t21 t22:t),
+        Node a1 e1 t11 t12 = Node a2 e2 t21 t22 ->
         a1 = a2.
     Proof
       let f a0 t :=
           match t with
-          | empty => a0
-          | node a e t1 t2 => a
+          | Empty => a0
+          | Node a e t1 t2 => a
           end
       in
       fun a1 a2 e1 e2 t11 t12 t21 t22 eq =>
@@ -151,14 +152,14 @@ Module Make (ElementM:ANY) (ExtraM:ANY).
           (f a1).
 
     Theorem node_injective_left_son:
-      forall (a1 a2:A) (e1 e2:E) (t11 t12 t21 t22:T),
-        node a1 e1 t11 t12 = node a2 e2 t21 t22 ->
+      forall (a1 a2:A.t) (e1 e2:E.t) (t11 t12 t21 t22:t),
+        Node a1 e1 t11 t12 = Node a2 e2 t21 t22 ->
         t11 = t21.
     Proof
       let f t0 t :=
           match t with
-          | empty => t0
-          | node a e t1 t2 => t1
+          | Empty => t0
+          | Node a e t1 t2 => t1
           end
       in
       fun a1 a2 e1 e2 t11 t12 t21 t22 eq =>
@@ -167,14 +168,14 @@ Module Make (ElementM:ANY) (ExtraM:ANY).
           (f t11).
 
     Theorem node_injective_right_son:
-      forall (a1 a2:A) (e1 e2:E) (t11 t12 t21 t22:T),
-        node a1 e1 t11 t12 = node a2 e2 t21 t22 ->
+      forall (a1 a2:A.t) (e1 e2:E.t) (t11 t12 t21 t22:t),
+        Node a1 e1 t11 t12 = Node a2 e2 t21 t22 ->
         t12 = t22.
     Proof
       let f t0 t :=
           match t with
-          | empty => t0
-          | node a e t1 t2 => t2
+          | Empty => t0
+          | Node a e t1 t2 => t2
           end
       in
       fun a1 a2 e1 e2 t11 t12 t21 t22 eq =>
@@ -189,26 +190,26 @@ Module Make (ElementM:ANY) (ExtraM:ANY).
   (** * Height                          *)
   (*====================================*)
   Section height.
-    Inductive Height: T -> nat -> Prop :=
+    Inductive Height: t -> nat -> Prop :=
     | empty_height:
-        Height empty 0
+        Height Empty 0
     | node_height:
         forall t1 h1 t2 h2 a i,
           Height t1 h1 ->
           Height t2 h2 ->
-          Height (node a i t1 t2) (1 + max h1 h2).
+          Height (Node a i t1 t2) (1 + max h1 h2).
 
-    Fixpoint height (t:T): nat :=
-      match t with
-      | empty => 0
-      | node _ _ t1 t2 =>
+    Fixpoint height (t_:t): nat :=
+      match t_ with
+      | Empty => 0
+      | Node _ _ t1 t2 =>
         1 + max (height t1) (height t2)
       end.
 
     Theorem height_is_only_height:
-      forall (t:T) (h:nat),
-        Height t h ->
-        h = height t.
+      forall (t_:t) (h:nat),
+        Height t_ h ->
+        h = height t_.
     Proof
       fix f t h ph :=
       match ph in Height t h
@@ -226,20 +227,20 @@ Module Make (ElementM:ANY) (ExtraM:ANY).
       end.
 
     Theorem height_is_height:
-      forall t:T, Height t (height t).
+      forall t_:t, Height t_ (height t_).
     Proof
       fix f t :=
       match t return Height t (height t) with
-      | empty =>
+      | Empty =>
         empty_height
-      | node a i t1 t2 =>
+      | Node a i t1 t2 =>
         node_height a i (f t1) (f t2)
       end.
 
     Theorem height_is_unique:
-      forall (t:T) (h1 h2:nat),
-        Height t h1 ->
-        Height t h2 ->
+      forall (t_:t) (h1 h2:nat),
+        Height t_ h1 ->
+        Height t_ h2 ->
         h1 = h2.
     Proof
       fix f t h1 h2 p1 p2 :=
@@ -256,40 +257,40 @@ Module Make (ElementM:ANY) (ExtraM:ANY).
   (** * Leftmost and Rightmost          *)
   (*====================================*)
   Section leftmost_and_rightmost.
-    Inductive Leftmost: T -> A -> Prop :=
+    Inductive Leftmost: t -> A.t -> Prop :=
     | lm_noleft:
-        forall a e t2, Leftmost (node a e empty t2) a
+        forall a e t2, Leftmost (Node a e Empty t2) a
     | lm_left:
         forall x a e t1 t2,
           Leftmost t1 x ->
-          Leftmost (node a e t1 t2) x.
+          Leftmost (Node a e t1 t2) x.
 
-    Inductive Rightmost: T -> A -> Prop :=
+    Inductive Rightmost: t -> A.t -> Prop :=
     | rm_noright:
-        forall a e t1, Rightmost (node a e t1 empty) a
+        forall a e t1, Rightmost (Node a e t1 Empty) a
     | rm_right:
         forall x a e t1 t2,
           Rightmost t2 x ->
-          Rightmost (node a e t1 t2) x.
+          Rightmost (Node a e t1 t2) x.
 
     Theorem leftmost_is_node:
-      forall (t:T) (a:A),
-        Leftmost t a -> Node t.
+      forall (t_:t) (a:A.t),
+        Leftmost t_ a -> is_Node t_.
     Proof
       fix f t a lm :=
       match lm in Leftmost t a
-            return Node t with
+            return is_Node t with
       | lm_noleft _ _ _ => I
       | lm_left _ _ _ _ => I
       end.
 
     Theorem rightmost_is_node:
-      forall (t:T) (a:A),
-        Rightmost t a -> Node t.
+      forall (t_:t) (a:A.t),
+        Rightmost t_ a -> is_Node t_.
     Proof
       fix f t a rm :=
       match rm in Rightmost t a
-            return Node t with
+            return is_Node t with
       | rm_noright _ _ _ => I
       | rm_right _ _ _ _ => I
       end.
@@ -297,39 +298,39 @@ Module Make (ElementM:ANY) (ExtraM:ANY).
 
 
 
-    Fixpoint leftmost (t:T): Node t -> A :=
-      match t return Node t -> A with
-      | empty =>
+    Fixpoint leftmost (t_:t): is_Node t_ -> A.t :=
+      match t_ return is_Node t_ -> A.t with
+      | Empty =>
         fun nd => match nd with end
-      | node a e t1 t2 =>
+      | Node a e t1 t2 =>
         match is_node t1 with
-        | left  nd => fun _ => leftmost t1 (nd:Node t1)
+        | left  nd => fun _ => leftmost t1 (nd:is_Node t1)
         | right _  => fun _ => a
         end
       end.
 
 
     Theorem leftmost_correct:
-      forall (t:T) (nd:Node t),
-        Leftmost t (leftmost t nd).
+      forall (t_:t) (nd:is_Node t_),
+        Leftmost t_ (leftmost t_ nd).
     Proof
       let P t nd := Leftmost t (leftmost t nd) in
       fix f t :=
       match t return forall nd, P t nd with
-      | empty => fun nd => match nd with end
-      | node a e t1 t2 =>
+      | Empty => fun nd => match nd with end
+      | Node a e t1 t2 =>
         fun nd =>
           (match t1
-                 return (forall nd1, P t1 nd1) -> P (node a e t1 t2) nd
+                 return (forall nd1, P t1 nd1) -> P (Node a e t1 t2) nd
            with
-           | empty =>
+           | Empty =>
              fun _ =>
                Equal.rewrite
-                 (Equal.flip eq_refl: a = leftmost (node a e empty t2) I)
-                 (fun x => Leftmost (node a e empty t2) x)
+                 (Equal.flip eq_refl: a = leftmost (Node a e Empty t2) I)
+                 (fun x => Leftmost (Node a e Empty t2) x)
                  (lm_noleft a e t2)
-           | node a1 e1 t11 t12 =>
-             let t1_ := node a1 e1 t11 t12 in
+           | Node a1 e1 t11 t12 =>
+             let t1_ := Node a1 e1 t11 t12 in
              fun p1: forall nd1, P t1_ nd1 =>
                @lm_left (leftmost t1_ I) a e t1_ t2 (p1 I)
            end) (f t1)
@@ -337,38 +338,38 @@ Module Make (ElementM:ANY) (ExtraM:ANY).
 
 
 
-    Fixpoint rightmost (t:T): Node t -> A :=
-      match t return Node t -> A with
-      | empty =>
+    Fixpoint rightmost (t_:t): is_Node t_ -> A.t :=
+      match t_ return is_Node t_ -> A.t with
+      | Empty =>
         fun nd => match nd with end
-      | node a e t1 t2 =>
+      | Node a e t1 t2 =>
         match is_node t2 with
-        | left  nd => fun _ => rightmost t2 (nd:Node t2)
+        | left  nd => fun _ => rightmost t2 (nd:is_Node t2)
         | right p  => fun _ => a
         end
       end.
 
     Theorem rightmost_correct:
-      forall (t:T) (nd:Node t),
-        Rightmost t (rightmost t nd).
+      forall (t_:t) (nd:is_Node t_),
+        Rightmost t_ (rightmost t_ nd).
     Proof
       let P t nd := Rightmost t (rightmost t nd) in
       fix f t :=
       match t return forall nd, P t nd with
-      | empty => fun nd => match nd with end
-      | node a e t1 t2 =>
+      | Empty => fun nd => match nd with end
+      | Node a e t1 t2 =>
         fun nd =>
           (match t2
-                 return (forall nd2, P t2 nd2) -> P (node a e t1 t2) nd
+                 return (forall nd2, P t2 nd2) -> P (Node a e t1 t2) nd
            with
-           | empty =>
+           | Empty =>
              fun _ =>
                Equal.rewrite
-                 (Equal.flip eq_refl: a = rightmost (node a e t1 empty) I)
-                 (fun x => Rightmost (node a e t1 empty) x)
+                 (Equal.flip eq_refl: a = rightmost (Node a e t1 Empty) I)
+                 (fun x => Rightmost (Node a e t1 Empty) x)
                  (rm_noright a e t1)
-           | node a2 e2 t21 t22 =>
-             let t2_ := node a2 e2 t21 t22 in
+           | Node a2 e2 t21 t22 =>
+             let t2_ := Node a2 e2 t21 t22 in
              fun p2: forall nd2, P t2_ nd2 =>
                @rm_right (rightmost t2_ I) a e t1 t2_ (p2 I)
            end) (f t2)
@@ -385,36 +386,36 @@ Module Make (ElementM:ANY) (ExtraM:ANY).
   (*====================================*)
   (* Inorder t xs:  'xs' is the inorder sequence of 't'.*)
   Section inorder_sequence.
-    Inductive Inorder: T -> list A -> Prop :=
-    | empty_inorder: Inorder empty []
+    Inductive Inorder: t -> list A.t -> Prop :=
+    | empty_inorder: Inorder Empty []
     | node_inorder:
         forall t1 xs1 t2 xs2 a e,
           Inorder t1 xs1 ->
           Inorder t2 xs2 ->
-          Inorder (node a e t1 t2) (xs1 ++ a :: xs2).
+          Inorder (Node a e t1 t2) (xs1 ++ a :: xs2).
 
-    Fixpoint inorder (t:T): list A :=
-      match t with
-      | empty => []
-      | node a e t1 t2 =>
+    Fixpoint inorder (t_:t): list A.t :=
+      match t_ with
+      | Empty => []
+      | Node a e t1 t2 =>
         inorder t1 ++ a :: inorder t2
       end.
 
 
     Theorem inorder_correct:
-      forall t:T, Inorder t (inorder t).
+      forall t_:t, Inorder t_ (inorder t_).
     Proof
       fix f t :=
       match t return Inorder t (inorder t) with
-      | empty => empty_inorder
-      | node a e t1 t2 =>
+      | Empty => empty_inorder
+      | Node a e t1 t2 =>
         @node_inorder t1 (inorder t1) t2 (inorder t2) a e (f t1) (f t2)
       end.
 
     Theorem inorder_unique:
-      forall (t:T) (xs:list A),
-        Inorder t xs ->
-        xs = inorder t.
+      forall (t_:t) (xs:list A.t),
+        Inorder t_ xs ->
+        xs = inorder t_.
     Proof
       fix f t xs ord :=
       match ord in Inorder t xs
